

Chapter I.1

The electromagnetic field

I.1.1 The electromagnetic four-tensor

The electromagnetic four tensor is, in terms of the electric/magnetic field

$$F^{\mu\nu} = \begin{bmatrix} 0 & -\frac{E_x}{c} & -\frac{E_y}{c} & -\frac{E_z}{c} \\ \frac{E_x}{c} & 0 & -B_z & B_y \\ \frac{E_y}{c} & B_z & 0 & -B_x \\ \frac{E_z}{c} & -B_y & B_x & 0 \end{bmatrix} \quad (\text{I.1.1})$$

Some constants in atomic units are

$$\hbar = 1, \quad e = -1, \quad c = 137.036, \quad m = 1 \quad (\text{I.1.2})$$

I.1.2 The plane wave

I.1.2.1 The field parameters

The field parameters are

1. ω = frequency. Typical values are $\omega = 0.05$ au
2. $n = (1, \mathbf{n})$ the propagation direction four-vector. Typically, $\mathbf{n} = \mathbf{e}_z$, i.e. the field propagates along Oz
3. $k = \frac{\omega}{c} n$
4. s the polarization four vector, $s \cdot n = 0$, $s^* \cdot s = -1$. Typically $s = (0, \mathbf{s})$, $\mathbf{s} \cdot \mathbf{s}^* = 1$, $\mathbf{s} \cdot \mathbf{n} = 0$. The choice for propagation direction along Oz is $s = (\zeta_x, \zeta_y, 0)$ with $|\zeta_x|^2 + |\zeta_y|^2 = 1$
5. the dimensionless intensity parameter $\xi = \frac{|e|A_0}{mc}$.

I.1.2.2 The electric field

$$E(x) = E_0 \Re \{ s e^{-i\phi - \frac{(\phi - \tau_0)^2}{\tau^2}} \}, \quad \phi \equiv k \cdot x = \omega t - \frac{\omega}{c} \mathbf{n} \cdot \mathbf{x} \quad (\text{I.1.3})$$

$\frac{\tau}{2\pi}$ is the length of the pulse measured in optical periods $T = \frac{2\pi}{\omega}$

The Cartesian components of the electric field are

$$E_x(\mathbf{r}, t) = E_0 \Re \{ \zeta_x f(\phi) \}, \quad f(\phi) = e^{-i\phi - \frac{(\phi - \tau_0)^2}{\tau^2}}, \quad \phi = \omega t - kz \quad (\text{I.1.4})$$

$$E_y(\mathbf{r}, t) = E_0 \Re \{ \zeta_y f(\phi) \} \quad (\text{I.1.5})$$

$$E_z(\mathbf{r}, t) = 0 \quad (\text{I.1.6})$$

I.1.2.3 The magnetic field

The magnetic field is

$$\mathbf{B}(x) = \frac{1}{c} \mathbf{n} \times \mathbf{E}(x) \quad (\text{I.1.7})$$

The Cartesian components of the magnetic field are

$$B_x(\mathbf{r}, t) = \frac{E_0}{c} \Re \{ -\zeta_y f(\phi) \}, \quad f(\phi) = e^{-i\phi - \frac{(\phi - \tau_0)^2}{\tau^2}}, \quad \phi = \omega t - kz \quad (\text{I.1.8})$$

$$B_y(\mathbf{r}, t) = \frac{E_0}{c} \Re \{ \zeta_x f(\phi) \} \quad (\text{I.1.9})$$

$$B_z(\mathbf{r}, t) = 0 \quad (\text{I.1.10})$$

I.1.3 The Laguerre Gauss modes

I.1.3.1 The field parameters

1. the dimensionless intensity parameter a_0 ; the amplitude of the electric field is $E_0 = \omega \xi \frac{mc}{|e|}$
2. propagation direction only along Oz axis. $\mathbf{n} = \mathbf{e}_z$
3. ω = frequency; $T = \frac{2\pi}{\omega}$, $k = \frac{\omega}{c}$, $\lambda = cT$
4. w_0 = the beam waist
5. $z_R = \frac{kw_0^2}{2}$ = the Rayleigh length
6. $w(z) = w_0 \sqrt{1 + \frac{z^2}{z_R^2}}$
7. $\psi_G(z) = \arctan \frac{z}{z_R}$
8. $\epsilon = \pm 1$ helicity sign
9. ζ_x, ζ_y polarization parameters $|\zeta_x|^2 + |\zeta_y|^2 = 1$

I.1.3.2 The scalar solution

Define the scalar solution

$$u_{pm}(\mathbf{r}) = N_{pm} \frac{w_0}{w(z)} \left(\frac{\sqrt{2}}{w(z)} \right)^m e^{-i(2p+m+1)\psi_G(z)} e^{-\frac{k}{2} \frac{x^2+y^2}{z_R+iz}} {}_1F_1(-p, m+1, \frac{2(x^2+y^2)}{w(z)^2})(x+i\epsilon y)^m \quad (\text{I.1.11})$$

The normalization constant is

$$N_{pm} = \frac{\sqrt{2}}{m!} \sqrt{\frac{(p+m)!}{p!}} \quad (\text{I.1.12})$$

The derivatives

$$\begin{aligned} \frac{du_{pm}(\mathbf{r})}{dx} = & N_{pm} \frac{w_0}{w(z)} \left(\frac{\sqrt{2}}{w(z)} \right)^m e^{-i(2p+m+1)\psi_G(z)} e^{-\frac{k}{2} \frac{x^2+y^2}{z_R+iz}} \\ & \times \left[{}_1F_1(-p, m+1, \frac{2(x^2+y^2)}{w(z)^2}) \left(m(x+i\epsilon y)^{m-1} - (x+i\epsilon y)^m \frac{kx}{z_R+iz} \right) \right. \\ & \left. - \frac{p}{m+1} \frac{4x}{w(z)^2} {}_1F_1(-p+1, m+2, \frac{2(x^2+y^2)}{w(z)^2}) \right] \end{aligned} \quad (\text{I.1.13})$$

$$\begin{aligned} \frac{du_{pm}(\mathbf{r})}{dy} = & N_{pm} \frac{w_0}{w(z)} \left(\frac{\sqrt{2}}{w(z)} \right)^m e^{-i(2p+m+1)\psi_G(z)} e^{-\frac{k}{2} \frac{x^2+y^2}{z_R+iz}} \\ & \times \left[{}_1F_1(-p, m+1, \frac{2(x^2+y^2)}{w(z)^2}) \left(im\epsilon(x+i\epsilon y)^{m-1} - (x+i\epsilon y)^m \frac{ky}{z_R+iz} \right) \right. \\ & \left. - \frac{p}{m+1} \frac{4y}{w(z)^2} {}_1F_1(-p+1, m+2, \frac{2(x^2+y^2)}{w(z)^2}) \right] \end{aligned} \quad (\text{I.1.14})$$

I.1.3.3 The electric field

The Cartesian components of the electric field are

$$E_x(\mathbf{r}, t) = E_0 \Re \left\{ \zeta_x u_{pm}(\mathbf{r}) f(\phi) \right\}, \quad f(\phi) = e^{-i\phi - \frac{(\phi-\tau_0)^2}{\tau^2}}, \quad \phi = \omega t - kz \quad (\text{I.1.15})$$

$$E_y(\mathbf{r}, t) = E_0 \Re \left\{ \zeta_y u_{pm}(\mathbf{r}) f(\phi) \right\} \quad (\text{I.1.16})$$

$$E_z(\mathbf{r}, t) = E_0 \Re \left\{ -\frac{1}{ik} \left[\zeta_x \frac{\partial u_{pm}(\mathbf{r})}{\partial x} + \zeta_y \frac{\partial u_{pm}(\mathbf{r})}{\partial y} \right] f(\phi) \right\} \quad (\text{I.1.17})$$

I.1.3.4 The magnetic field

The Cartesian components of the magnetic field are

$$B_x(\mathbf{r}, t) = \frac{E_0}{c} \Re \left\{ -\zeta_y u_{pm}(\mathbf{r}) f(\phi) \right\}, \quad f(\phi) = e^{-i\phi - \frac{(\phi-\tau)^2}{\tau^2}}, \quad \phi = \omega t - kz \quad (\text{I.1.18})$$

$$B_y(\mathbf{r}, t) = \frac{E_0}{c} \Re \left\{ \zeta_x u_{pm}(\mathbf{r}) f(\phi) \right\} \quad (\text{I.1.19})$$

$$B_z(\mathbf{r}, t) = \frac{E_0}{c} \Re \left\{ -\frac{1}{ik} \left[-\zeta_y \frac{\partial u_{pm}(\mathbf{r})}{\partial x} + \zeta_x \frac{\partial u_{pm}(\mathbf{r})}{\partial y} \right] f(\phi) \right\} \quad (\text{I.1.20})$$

Chapter I.2

The classical motion of a charged particle in the electromagnetic field

I.2.1 The relation between covariant and non-covariant velocity/acceleration

I.2.1.1 The covariant kinematics

The independent variable is the proper time of the particle τ

1. the trajectory

$$r(\tau) \equiv (ct(\tau), x(\tau), y(\tau), z(\tau)) \quad (\text{I.2.1})$$

2. the 4-velocity

$$u(\tau) = \frac{dr(\tau)}{d\tau}, \quad u \cdot u = c^2 \quad (\text{I.2.2})$$

3. the 4-acceleration

$$\rho(\tau) = \frac{du(\tau)}{d\tau}, \quad \rho \cdot u = 0 \quad (\text{I.2.3})$$

I.2.1.2 The non-covariant kinematics

The independent variable is the laboratory time t . The relation between the proper time τ and the laboratory time t is

$$dt = \gamma d\tau, \quad \gamma = \frac{1}{\sqrt{1 - \frac{v^2}{c^2}}} = \frac{u^0}{c}, \quad \frac{d}{d\tau} = \frac{1}{\gamma} \frac{d}{dt} \quad (\text{I.2.4})$$

1. the trajectory

$$r(t) \equiv (x(t), y(t), z(t)) \quad (\text{I.2.5})$$

2. the velocity

$$v(t) = \frac{dr(t)}{dt}, \quad v(t) = \frac{u}{\gamma} = c \frac{u}{u^0}, \quad \beta = \frac{v}{c} = \frac{u}{u^0} \quad (\text{I.2.6})$$

3. the acceleration

$$\mathbf{a}(t) = \frac{d\mathbf{v}(t)}{dt} = \frac{d}{dt} \frac{\mathbf{u}}{\gamma} = \frac{1}{\gamma} \frac{d\mathbf{u}}{dt} - \mathbf{u} \frac{1}{\gamma^2} \frac{d\gamma}{dt} = \frac{1}{\gamma^2} \frac{d\mathbf{u}}{d\tau} - \mathbf{u} \frac{1}{\gamma^3} \frac{d\gamma}{d\tau} = \frac{1}{\gamma^2} \boldsymbol{\rho} - \mathbf{u} \frac{1}{\gamma^3} \frac{d\gamma}{d\tau} \quad (\text{I.2.7})$$

From

$$\gamma = \frac{1}{c} \sqrt{c^2 + \mathbf{u}^2} \quad \longrightarrow \quad \frac{d\gamma}{d\tau} = \frac{1}{c \sqrt{c^2 + \mathbf{u}^2}} \mathbf{u} \cdot \frac{d\mathbf{u}}{d\tau} = \frac{1}{c^2 \gamma} \mathbf{u} \cdot \boldsymbol{\rho} \quad (\text{I.2.8})$$

and the acceleration is

$$\mathbf{a}(t) = \frac{1}{\gamma^2} \boldsymbol{\rho} - \frac{1}{c^2 \gamma^4} (\mathbf{u} \cdot \boldsymbol{\rho}) \mathbf{u} = \frac{1}{\gamma^2} \left(\boldsymbol{\rho} - \frac{1}{c^2} (\mathbf{v} \cdot \boldsymbol{\rho}) \mathbf{v} \right) = \frac{1}{\gamma^2} (\boldsymbol{\rho} - (\boldsymbol{\beta} \cdot \boldsymbol{\rho}) \boldsymbol{\beta}) \quad (\text{I.2.9})$$

$$\dot{\boldsymbol{\beta}}(t) \equiv \frac{d\boldsymbol{\beta}(t)}{dt} = \frac{1}{\gamma^2 c} (\boldsymbol{\rho} - (\boldsymbol{\beta} \cdot \boldsymbol{\rho}) \boldsymbol{\beta}) \quad (\text{I.2.10})$$

I.2.2 The covariant equations of motion

The equation of motion of a charged particle in the field is

$$\frac{dx^\mu}{d\tau} = u^\mu, \quad \frac{du^\mu}{d\tau} = \frac{e}{m} F^{\mu\nu} u_\nu \quad (\text{I.2.11})$$

where τ is the proper time.

I.2.3 The non-covariant equations

The derivatives of the coordinates are

$$\frac{d\mathbf{x}}{dt} = \frac{1}{\gamma} d\mathbf{x} d\tau = c \frac{\mathbf{u}}{u^0} = \mathbf{v} = c \boldsymbol{\beta} \quad (\text{I.2.12})$$

Using the explicit form of F we obtain

$$m \frac{d}{dt} (\gamma \mathbf{v}) = e (\mathbf{E} + \mathbf{v} \times \mathbf{B}) \quad (\text{I.2.13})$$

i.e.

$$m \frac{d\gamma}{dt} \mathbf{v} + m \gamma \frac{d\mathbf{v}}{dt} = e (\mathbf{E} + \mathbf{v} \times \mathbf{B}) \quad (\text{I.2.14})$$

We multiply the entire equation by \mathbf{v} and we get

$$m \frac{d\gamma}{dt} \mathbf{v}^2 + m \gamma \mathbf{v} \cdot \frac{d\mathbf{v}}{dt} = e \mathbf{E} \cdot \mathbf{v}, \quad m \frac{d\gamma}{dt} \mathbf{v}^2 + m \gamma \frac{1}{2} \frac{d\mathbf{v}^2}{dt} = e \mathbf{E} \cdot \mathbf{v}, \quad (\text{I.2.15})$$

Using the definition of γ

$$\gamma = \frac{1}{\sqrt{1 - \frac{\mathbf{v}^2}{c^2}}}, \quad \longrightarrow \quad \frac{d\gamma}{dt} = \frac{1}{2} \frac{\gamma^3}{c^2} \frac{d\mathbf{v}^2}{dt} \quad \longrightarrow \quad \frac{d\mathbf{v}^2}{dt} = \frac{2c^2}{\gamma^3} \frac{d\gamma}{dt}, \quad \mathbf{v}^2 = c^2 \frac{\gamma^2 - 1}{\gamma^2} \quad (\text{I.2.16})$$

Finally, we have

$$m \frac{d\gamma}{dt} c^2 \frac{\gamma^2 - 1}{\gamma^2} + m \gamma \frac{1}{2} \frac{2c^2}{\gamma^3} \frac{d\gamma}{dt} = e \mathbf{E} \cdot \mathbf{v}, \quad m c^2 \frac{d\gamma}{dt} = e \mathbf{E} \cdot \mathbf{v} \quad (\text{I.2.17})$$

and the second equation of motion becomes

$$\frac{e\mathbf{E} \cdot \mathbf{v}}{c^2} \mathbf{v} + m\gamma \frac{d\mathbf{v}}{dt} = e(\mathbf{E} + \mathbf{v} \times \mathbf{B}) \quad (\text{I.2.18})$$

i.e.

$$m\gamma \frac{d\mathbf{v}}{dt} = e \left(\mathbf{E} + \mathbf{v} \times \mathbf{B} - \frac{1}{c^2} (\mathbf{E} \cdot \mathbf{v}) \mathbf{v} \right) \quad (\text{I.2.19})$$

The system of 6 equations that has to be solved numerically is

$$\frac{d\mathbf{r}}{dt} = \mathbf{v} \quad (\text{I.2.20})$$

$$\frac{d\mathbf{v}}{dt} = \frac{e}{m\gamma} \left(\mathbf{E} + \mathbf{v} \times \mathbf{B} - \frac{1}{c^2} (\mathbf{E} \cdot \mathbf{v}) \mathbf{v} \right), \quad \gamma = \frac{1}{\sqrt{1 - \frac{v^2}{c^2}}} \quad (\text{I.2.21})$$

Chapter I.3

The ponderomotive force theory

I.3.1 Equations of motion

Consider the relativistic equations of motion for a particle with a time and coordinate dependent mass $\mathcal{M}(\mathbf{x}, t)$
The covariant Lagrange function will be

$$L_{(\tau)} = -\mathcal{M}(x)c\sqrt{\frac{dx_\mu}{d\tau}\frac{dx^\mu}{d\tau}} = -\mathcal{M}(x)c\sqrt{\dot{x}_\mu\dot{x}^\mu} \quad (\text{I.3.1})$$

The equations of motion are obtained from

$$\frac{\partial L_{(\tau)}}{\partial \dot{x}_\mu} = -\mathcal{M}(x)c\frac{\dot{x}^\mu}{\sqrt{\dot{x}_\mu\dot{x}^\mu}} \quad \frac{\partial L_{(\tau)}}{\partial x_\mu} = -\frac{\partial \mathcal{M}(x)}{\partial x_\mu}c\sqrt{\dot{x}_\mu\dot{x}^\mu}, \quad (\text{I.3.2})$$

$$\frac{d}{d\tau} \left(-\mathcal{M}(x)c\frac{\dot{x}^\mu}{\sqrt{\dot{x}_\mu\dot{x}^\mu}} \right) = -\frac{\partial \mathcal{M}(x)}{\partial x_\mu}c\sqrt{\dot{x}_\mu\dot{x}^\mu} \quad (\text{I.3.3})$$

If we assume that

$$\dot{x}_\mu\dot{x}^\mu = c^2 \quad (\text{I.3.4})$$

as it should be then the equations of motion are

$$\frac{d}{d\tau} (\mathcal{M}(x)\dot{x}^\mu) = c^2 \frac{\partial \mathcal{M}(x)}{\partial x_\mu} \quad (\text{I.3.5})$$

The expression of the four acceleration $\frac{du}{d\tau}$ will be

$$\mathcal{M}(x)\frac{d\dot{x}^\mu}{d\tau} = c^2 \frac{\partial \mathcal{M}(x)}{\partial x_\mu} - \dot{x}^\mu \frac{d\mathcal{M}(x)}{d\tau} = c^2 \frac{\partial \mathcal{M}(x)}{\partial x_\mu} - \dot{x}^\mu \dot{x}^\nu \frac{\partial \mathcal{M}(x)}{\partial x^\nu} = (c^2 g^{\mu\nu} - \dot{x}^\mu \dot{x}^\nu) \frac{\partial \mathcal{M}(x)}{\partial x^\nu} \quad (\text{I.3.6})$$

The covariant form of the equations of motion

$$\boxed{\frac{dx^\mu}{d\tau} = u^\mu, \quad \frac{du^\mu}{d\tau} = \frac{1}{\mathcal{M}(x)} (c^2 g^{\mu\nu} - \dot{x}^\mu \dot{x}^\nu) \frac{\partial \mathcal{M}(x)}{\partial x^\nu}} \quad (\text{I.3.7})$$

To check the correctness of the above formula we should verify that

$$u \cdot \frac{du}{d\tau} = 0 \quad (\text{I.3.8})$$

In our case,

$$u_\mu \frac{du^\mu}{d\tau} = \frac{1}{\mathcal{M}(x)} (c^2 g^{\mu\nu} - u^\mu u^\nu) u_\mu \frac{\partial \mathcal{M}(x)}{\partial x^\nu} = 0 \quad (\text{I.3.9})$$

The above formulas are valid if $u^\mu \approx 0$, or $u^\mu \ll c$. If u is not small, the formulas are still valid, but in a reference frame in which the dressed electron is at rest, and we need to perform a Lorentz boost to find the acceleration in the laboratory frame.

I.3.2 The dressed mass

In our case we define the variable mass in terms of a 4-vector potential

$$A(x) = \left(\frac{\Phi(x)}{c}, \mathbf{A}(x) \right) \quad (\text{I.3.10})$$

as

$$\mathcal{M}(x) = m \sqrt{1 - \frac{e^2 \langle A^2 \rangle(x)}{(mc)^2}} \quad (\text{I.3.11})$$

where m is the (constant) mass of the isolated particle and $\langle A^2 \rangle(x)$ is the time average

$$\langle A^2 \rangle(x) = \frac{1}{T} \int_{-T/2}^{T/2} d\tau A^2(t + \tau, \mathbf{x}) \quad (\text{I.3.12})$$

In a Coulomb gauge, the four vector potential reduces to

$$A(x) = (0, \mathbf{A}(x)), \quad A^2(x) = -\mathbf{A}^2(x) \quad (\text{I.3.13})$$

and the dressed mass becomes

$$\mathcal{M}(x) = m \sqrt{1 + \frac{e^2 \langle \mathbf{A}^2 \rangle(x)}{(mc)^2}}, \quad \langle \mathbf{A}^2 \rangle(x) = \frac{1}{T} \int_{-T/2}^{T/2} d\tau \mathbf{A}^2(t + \tau, \mathbf{x}) = -\frac{1}{T} \int_{-T/2}^{T/2} d\tau A^2(t + \tau, \mathbf{x}) \quad (\text{I.3.14})$$

Define the dimensionless quantity

$$a(x) = \frac{e^2}{(mc)^2} \frac{1}{T} \int_{-T/2}^{T/2} d\tau \mathbf{A}^2(t + \tau, \mathbf{x}) = -\frac{e^2}{(mc)^2} \frac{1}{T} \int_{-T/2}^{T/2} d\tau A^2(t + \tau, \mathbf{x}) \quad (\text{I.3.15})$$

The derivatives are

$$\frac{\partial a(x)}{\partial x_\mu} = \frac{2e^2}{(mc)^2} \frac{1}{T} \int_{-T/2}^{T/2} d\tau \mathbf{A}(t + \tau, \mathbf{x}) \cdot \partial^\mu \mathbf{A}(t + \tau, \mathbf{x}) = -\frac{2e^2}{(mc)^2} \frac{1}{T} \int_{-T/2}^{T/2} d\tau \mathbf{A}(t + \tau, \mathbf{x}) \cdot \partial^\mu A(t + \tau, \mathbf{x}) \quad (\text{I.3.16})$$

We can define the 4-vector

$$v = (1, 0, 0, 0), \quad \text{and} \quad c\tau v = (c\tau, 0, 0, 0) \quad (\text{I.3.17})$$

and define A as a function of the four-vector $x \equiv (ct, \mathbf{x})$. Then in covariant notations we get

$$a(x) = -\frac{e^2}{(mc)^2} \frac{1}{\lambda} \int_{-\lambda/2}^{\lambda/2} d\chi A^2(x + \chi v) = -\frac{e^2}{(mc)^2} \frac{1}{\lambda} \int_{-\lambda/2}^{\lambda/2} d\chi A_\alpha(x + \chi v) A^\alpha(x + \chi v) \quad (\text{I.3.18})$$

$$\partial^\mu a(x) = -\frac{2e^2}{(mc)^2} \frac{1}{\lambda} \int_{-\lambda/2}^{\lambda/2} d\chi A(x + \chi v) \cdot \partial^\mu A(x + \chi v) = -\frac{2e^2}{(mc)^2} \frac{1}{\lambda} \int_{-\lambda/2}^{\lambda/2} d\chi A_\alpha(x + \chi v) \cdot \partial^\mu A^\alpha(x + \chi v) \quad (\text{I.3.19})$$

$$\mathcal{M}(x) = m\sqrt{1 + a(x)} \quad (\text{I.3.20})$$

$$\partial^\mu \mathcal{M}(x) = m\partial^\mu \sqrt{1 + a(x)} = \frac{m}{2} \partial^\mu a(x) \frac{1}{\sqrt{1 + a(x)}} \quad (\text{I.3.21})$$

Appendix A

Elements of relativistic dynamics

A.1 The relativistic Lagrangian theory for a particle in a potential force

For a particle of mass m , moving in a potential field

$$V(\mathbf{x}) \tag{A.1}$$

the Lagrange (non-covariant) function is

$$L_{(t)} = -mc\sqrt{c^2 - \mathbf{v}^2(t)} - V(\mathbf{x}) \tag{A.2}$$

where

$$\mathbf{v}(t) = \frac{d\mathbf{x}(t)}{dt} \tag{A.3}$$

is the non-covariant velocity. The action integral is

$$S = \int_{t_1}^{t_2} dt L_{(t)} \tag{A.4}$$

and the extremum condition for the action becomes

$$\begin{aligned} \delta S &= \delta \int_{t_1}^{t_2} dt L_{(t)}(\mathbf{x}, \mathbf{v}) = \int_{t_1}^{t_2} dt \left(\frac{\partial L}{\partial \mathbf{x}} \cdot \delta \mathbf{x} + \frac{\partial L}{\partial \mathbf{v}} \cdot \delta \mathbf{v} \right) = \int_{t_1}^{t_2} dt \left(\frac{\partial L}{\partial \mathbf{x}} \cdot \delta \mathbf{x} + \frac{\partial L}{\partial \mathbf{v}} \cdot \delta \frac{d\mathbf{x}}{dt} \right) = \int_{t_1}^{t_2} dt \left(\frac{\partial L}{\partial \mathbf{x}} \cdot \delta \mathbf{x} + \frac{\partial L}{\partial \mathbf{v}} \cdot \frac{d\delta \mathbf{x}}{dt} \right) = \\ &= \int_{t_1}^{t_2} dt \left(\frac{\partial L}{\partial \mathbf{x}} \cdot \delta \mathbf{x} + \frac{d}{dt} \left(\frac{\partial L}{\partial \mathbf{v}} \cdot \delta \mathbf{x} \right) - \frac{d}{dt} \left(\frac{\partial L}{\partial \mathbf{v}} \right) \cdot \delta \mathbf{x} \right) = \int_{t_1}^{t_2} dt \left(\frac{\partial L}{\partial \mathbf{x}} - \frac{d}{dt} \frac{\partial L}{\partial \mathbf{v}} \right) \cdot \delta \mathbf{x} \end{aligned} \tag{A.5}$$

The Lagrange equations become

$$\frac{\partial L_{(t)}}{\partial \mathbf{x}} - \frac{d}{dt} \frac{\partial L_{(t)}}{\partial \mathbf{v}} = \mathbf{0} \tag{A.6}$$

i.e.

$$-\frac{\partial V}{\partial \mathbf{x}} = \frac{d}{dt} \frac{mc\mathbf{v}}{\sqrt{c^2 - \mathbf{v}^2}} \tag{A.7}$$

The relativistic momentum is

$$\mathbf{p} = \frac{\partial L_{(t)}}{\partial \mathbf{v}} = \frac{mc\mathbf{v}}{\sqrt{c^2 - v^2}} = \frac{m\mathbf{v}}{\sqrt{1 - \frac{v^2}{c^2}}} = m\gamma\mathbf{v} \quad (\text{A.8})$$

and the three dimensional force acting on the particle is

$$\mathbf{F} = -\frac{\partial V(\mathbf{x})}{\partial \mathbf{x}} \quad (\text{A.9})$$

and we obtained the equation of motion in the non-covariant form

$$\mathbf{F} = -\frac{\partial V}{\partial \mathbf{x}} = \frac{d\mathbf{p}}{dt}, \quad \mathbf{p} = m\gamma\mathbf{v} \quad (\text{A.10})$$

$$\boxed{\frac{d\mathbf{x}}{dt} = \mathbf{v}, \quad \frac{d}{dt}(m\gamma\mathbf{v}) = \mathbf{F} = -\frac{\partial V}{\partial \mathbf{x}}} \quad (\text{A.11})$$

To get the covariant version of the equation of motion we define the proper time τ , with

$$dt = \gamma d\tau, \quad d\tau = \frac{dt}{\gamma}, \quad \frac{d}{d\tau} = \gamma \frac{d}{dt} \quad (\text{A.12})$$

and

$$x = (ct, \mathbf{x}), \quad u = \frac{dx}{d\tau} = (\gamma c, \gamma\mathbf{v}), \quad \mathbf{p} = m\mathbf{u} = (\gamma mc, \gamma\mathbf{v}) = (mc\gamma, \mathbf{p}) \quad (\text{A.13})$$

The four vector force is

$$K = \frac{d\mathbf{p}}{d\tau} = \left(mc \frac{d\gamma}{d\tau}, \frac{d\mathbf{p}}{d\tau} \right) \quad (\text{A.14})$$

The derivative of γ is calculated directly

$$\frac{d\gamma}{dt} = \frac{d}{dt} \frac{1}{\sqrt{1 - \frac{v^2}{c^2}}} = \frac{1}{c^2} \frac{\mathbf{v} \cdot \frac{d\mathbf{v}}{dt}}{(1 - \frac{v^2}{c^2})^{3/2}} \quad (\text{A.15})$$

and

$$\frac{d\gamma}{dt} = \frac{\gamma^3}{c^2} \mathbf{v} \cdot \frac{d\mathbf{v}}{dt}, \quad mc \frac{d\gamma}{d\tau} = \gamma^4 \frac{m}{c} \mathbf{v} \cdot \frac{d\mathbf{v}}{dt} \quad (\text{A.16})$$

We want to prove that the four-force K is orthogonal on the four velocity u , i.e.

$$mc \frac{d\gamma}{d\tau} c\gamma = \frac{d\mathbf{p}}{d\tau} \cdot \gamma\mathbf{v} = m \frac{d\gamma\mathbf{v}}{d\tau} \cdot \gamma\mathbf{v} \quad (\text{A.17})$$

A direct proof is obvious, i.e.

$$m \frac{1}{2} \frac{d}{d\tau} (c^2 \gamma^2) - m \frac{1}{2} \frac{d}{d\tau} (\gamma\mathbf{v})^2 = \frac{m}{2} \frac{d}{d\tau} (\gamma^2 (c^2 - v^2)) = \frac{mc^2}{2} \frac{d}{d\tau} 1 = 0 \quad (\text{A.18})$$

A more involved proof would be

$$mc \frac{d\gamma}{d\tau} = \frac{1}{c\gamma} \frac{d\mathbf{p}}{d\tau} \cdot \gamma\mathbf{v} = \frac{\gamma}{c} \frac{d\mathbf{p}}{dt} \cdot \mathbf{v} = m \frac{\gamma}{c} \frac{d\gamma\mathbf{v}}{dt} \cdot \mathbf{v} = m \frac{\gamma}{c} \left(\frac{d\gamma}{dt} v^2 + \gamma \frac{d\mathbf{v}}{dt} \cdot \mathbf{v} \right) \quad (\text{A.19})$$

or

$$mc\gamma \frac{d\gamma}{dt} = m\frac{\gamma}{c} \left(\frac{d\gamma}{dt} v^2 + \gamma \frac{d\mathbf{v}}{dt} \cdot \mathbf{v} \right), \quad \frac{d\gamma}{dt} = \frac{1}{c^2} \left(\frac{d\gamma}{dt} v^2 + \gamma \frac{d\mathbf{v}}{dt} \cdot \mathbf{v} \right), \quad \frac{1}{\gamma^2} \frac{d\gamma}{dt} = \frac{1}{c^2} \gamma \frac{d\mathbf{v}}{dt} \cdot \mathbf{v} \quad (\text{A.20})$$

which is equivalent to the result (A.16).

The covariant version of the equation of motion is

$$x = (ct, \mathbf{x}), \quad \frac{dx}{d\tau} = u, \quad \frac{d(mu)}{d\tau} = K, \quad K = \left(\gamma \frac{\mathbf{v}}{c} \cdot \mathbf{F}, \gamma F \right) = \left(\frac{\mathbf{u}}{c} \cdot \mathbf{F}, \frac{u^0}{c} F \right), \quad \mathbf{F} = -\frac{\partial V}{\partial \mathbf{x}} \quad (\text{A.21})$$

or

$$\boxed{x = (ct, \mathbf{x}), \quad \frac{dx}{d\tau} = \frac{\mathbf{p}}{m}, \quad \frac{dp}{d\tau} = K, \quad K = \left(\frac{\mathbf{p}}{mc} \cdot \mathbf{F}, \frac{p^0}{mc} F \right), \quad \mathbf{F} = -\frac{\partial V}{\partial \mathbf{x}}} \quad (\text{A.22})$$

The direct derivation of the above equations can be obtained directly from the covariant Lagrange function. The action integral can be written as

$$S = \int dt L_{(t)} = \int d\tau \gamma L_{(t)} = \int d\tau L_{(\tau)}, \quad L_{(\tau)} = \gamma L_{(t)} = -mc\gamma \sqrt{c^2 - \mathbf{v}^2} - \gamma V(\mathbf{x}) \quad (\text{A.23})$$

i.e.

$$L_{(\tau)} = -mc \sqrt{\frac{dx_\mu}{d\tau} \frac{dx^\mu}{d\tau}} - \frac{1}{c} \frac{dx^0}{d\tau} V(\mathbf{x}) \quad (\text{A.24})$$

The covariant equations of motion are

$$\frac{d}{d\tau} \frac{\partial L_{(\tau)}}{\partial \dot{x}_\mu} = \frac{\partial L_{(\tau)}}{\partial x_\mu}, \quad \dot{x}_\mu = \frac{dx_\mu}{d\tau} \quad (\text{A.25})$$

In our case

$$\frac{\partial L_{(\tau)}}{\partial \dot{x}_i} = -m\dot{x}^i, \quad \frac{\partial L_{(\tau)}}{\partial x_i} = -\frac{1}{c} \dot{x}^0 \frac{\partial V}{\partial x_i} = \frac{1}{c} \dot{x}^0 \frac{\partial V(\mathbf{x})}{\partial x^i} = -\gamma F^i = -K^i \quad (\text{A.26})$$

and the spatial components of the equations of motions become

$$\frac{d}{d\tau} (m\dot{x}^i) = K^i \quad (\text{A.27})$$

for the temporal components we get

$$\frac{\partial L_{(\tau)}}{\partial \dot{x}_0} = -mc\dot{x}^0 - \frac{1}{c} V(\mathbf{x}), \quad \frac{d}{d\tau} \frac{\partial L_{(\tau)}}{\partial \dot{x}_0} = -mc \frac{d\dot{x}^0}{d\tau} - \frac{1}{c} \frac{\partial V}{\partial x^i} \dot{x}^i = -mc \frac{d\dot{x}^0}{d\tau} + \frac{1}{c} \mathbf{F} \cdot \mathbf{u} \quad (\text{A.28})$$

i.e.

$$mc \frac{du^0}{d\tau} = \frac{1}{c} \mathbf{F} \cdot \mathbf{u} \quad (\text{A.29})$$

with the notation

$$u = \dot{x}, \quad p = mu \quad (\text{A.30})$$

we get

$$\boxed{\dot{x} = u = \frac{\mathbf{p}}{m}, \quad \dot{p} = K, \quad K = \left(\frac{1}{cm} \mathbf{F} \cdot \mathbf{p}, \frac{p^0}{mc} F \right), \quad F^i = -\frac{\partial V(\mathbf{x})}{\partial x^i}} \quad (\text{A.31})$$

A.2 The relativistic Lagrangian theory for a particle in an electromagnetic field

In that case the potential is

$$V(x, \dot{x}) = q \left(\frac{\Phi}{c} - \mathbf{A} \cdot \mathbf{v} \right) \quad (\text{A.32})$$

and the covariant Lagrange function

$$L_{(\tau)} = -mc \sqrt{\frac{dx_\mu}{d\tau} \frac{dx^\mu}{d\tau}} - \frac{1}{c} \frac{dx^0}{d\tau} V(x, \dot{x}) = -mc \sqrt{\frac{dx_\mu}{d\tau} \frac{dx^\mu}{d\tau}} - q A_\mu(x) \cdot \frac{dx_\mu}{d\tau} \quad (\text{A.33})$$

where A is the four potential

$$A(x) = \left(\frac{\Phi(x)}{c}, \mathbf{A}(x) \right) \quad (\text{A.34})$$

Then the covariant Lagrange equations become

$$\frac{\partial L_{(\tau)}}{\partial \left(\frac{dx^\mu}{d\tau} \right)} = -m \frac{dx_\mu}{d\tau} - q A_\mu(x), \quad \frac{d}{d\tau} \frac{\partial L_{(\tau)}}{\partial \left(\frac{dx^\mu}{d\tau} \right)} = -m \frac{d}{d\tau} \frac{dx_\mu}{d\tau} - q \partial_\nu A_\mu(x) \frac{dx_\nu}{d\tau} \quad (\text{A.35})$$

$$\frac{\partial L_{(\tau)}}{\partial x^\mu} = -q \partial_\mu A_\nu \frac{dx^\nu}{d\tau} \quad (\text{A.36})$$

$$\frac{d}{d\tau} \left(m \frac{dx_\mu}{d\tau} \right) = q \left(\partial_\mu A_\nu(x) - \partial_\nu A_\mu(x) \right) \frac{dx^\nu}{d\tau} \quad (\text{A.37})$$

or

$$\boxed{\frac{dx^\mu}{d\tau} = \frac{p^\mu}{m}} \quad (\text{A.38})$$

$$\boxed{\frac{dp^\mu}{d\tau} = \frac{q}{m} F^{\mu\nu}(x) p_\nu, \quad F_{\mu\nu}(x) = \partial_\mu A_\nu(x) - \partial_\nu A_\mu(x)} \quad (\text{A.39})$$